src/array/Array_checker.v
@@ -101,6 +101,23 @@ Section certif.
     end.
 
 
+
+  Definition eq_sel_sym ti te a b sela selb :=
+    match get_atom sela, get_atom selb with
+    | Abop (BO_select ti1 te1) a' d1, Abop (BO_select ti2 te2) b' d2 =>
+      Typ.eqb ti ti1 && Typ.eqb ti ti2 &&
+      Typ.eqb te te1 && Typ.eqb te te2 &&
+      (a == a') && (b == b') && (d1 == d2) &&
+      match get_atom d1 with
+      | Abop (BO_diffarray ti3 te3) a3 b3 =>
+        Typ.eqb ti ti3 && Typ.eqb te te3 &&
+        (a3 == a) && (b3 == b)
+      | _ => false
+      end
+    | _, _ => false
+    end.
+  
+  
   Definition check_ext lres :=
     if Lit.is_pos lres then
       match get_form (Lit.blit lres) with
@@ -113,23 +130,9 @@ Section certif.
             | Fatom eqa, Fatom eqsel =>
               match get_atom eqa, get_atom eqsel with
               | Abop (BO_eq (Typ.TFArray ti te)) a b, Abop (BO_eq te') sela selb => 
-                if Typ.eqb te te' then
-                  match get_atom sela, get_atom selb with
-                  | Abop (BO_select ti1 te1) a' d1, Abop (BO_select ti2 te2) b' d2 =>
-                    if Typ.eqb ti ti1 && Typ.eqb ti ti2 &&
-                       Typ.eqb te te1 && Typ.eqb te te2 &&
-                       (a == a') && (b == b') && (d1 == d2) then
-                      match get_atom d1 with
-                      | Abop (BO_diffarray ti3 te3) a3 b3 =>
-                        if Typ.eqb ti ti3 && Typ.eqb te te3 &&
-                           (a3 == a) && (b3 == b) then
-                          lres :: nil
-                        else C._true
-                      | _ => C._true
-                      end
-                    else C._true
-                  | _, _ => C._true
-                  end
+                if Typ.eqb te te' && (eq_sel_sym ti te a b sela selb ||
+                                      eq_sel_sym ti te b a sela selb) then
+                  lres :: nil
                 else C._true
               | _, _ => C._true
               end
@@ -902,403 +905,376 @@ Section certif.
     afold_left bool int false orb (Lit.interp rho) a =
     C.interp rho (to_list a).
 
-Require Import Psatz.
+  Require Import Psatz.
 
-    Lemma valid_check_ext lres : C.valid rho (check_ext lres).
-      unfold check_ext.
-      case_eq (Lit.is_pos lres); intro Heq; simpl; try now apply C.interp_true.
-      case_eq (t_form .[ Lit.blit lres]); try (intros; now apply C.interp_true).
-      intros a Heq2.
-      case_eq (length a == 2); [ intros Heq3 | intros Heq3; now apply C.interp_true].
-      case_eq (Lit.is_pos (a .[ 0]) && negb (Lit.is_pos (a .[ 1])));
-        [ intros Heq4 | intros Heq4; now apply C.interp_true].
-      case_eq (t_form .[ Lit.blit (a .[0])]); try (intros; now apply C.interp_true).
-      intros b Heq5.
-      case_eq (t_form .[ Lit.blit (a .[1])]); try (intros; now apply C.interp_true).
-      intros c Heq6.
-      case_eq (t_atom .[ b]); try (intros; now apply C.interp_true).
-      intros [ | | | | | | | |N|N|N|N|N|N|N|N|N| | | | ] b1 b2 Heq7; try (intros; now apply C.interp_true).
-      case_eq t; try (intros; now apply C.interp_true). intros t0 t1 Heq8.
-      case_eq (t_atom .[ c]); try (intros; now apply C.interp_true).
-      intros [ | | | | | | | |N|N|N|N|N|N|N|N|N| | | | ] c1 c2 Heq9; try (intros; now apply C.interp_true).
-      case_eq (Typ.eqb t1 t2); [ intros Heq10 | intros Heq10; now apply C.interp_true].
-      case_eq (t_atom .[ c1]); try (intros; now apply C.interp_true).
-      intros [ | | | | | | | |N|N|N|N|N|N|N|N|N| | | | ] d1 d2 Heq11; try (intros; now apply C.interp_true).
-      case_eq (t_atom .[ c2]); try (intros; now apply C.interp_true).
-      intros [ | | | | | | | |N|N|N|N|N|N|N|N|N| | | | ] e1 e2 Heq12; try (intros; now apply C.interp_true).
-      case_eq (Typ.eqb t0 t3 && Typ.eqb t0 t5 && Typ.eqb t1 t4 && Typ.eqb t1 t6 && 
-                  (b1 == d1) && (b2 == e1) && (d2 == e2)); 
-                  [ intros Heq13 | intros Heq13; now apply C.interp_true].
-      case_eq (t_atom .[ d2]); try (intros; now apply C.interp_true).
-      intros [ | | | | | | | |N|N|N|N|N|N|N|N|N| | | | ] f1 f2 Heq14; try (intros; now apply C.interp_true).
+  Lemma valid_check_ext lres : C.valid rho (check_ext lres).
+    unfold check_ext, eq_sel_sym.
+    case_eq (Lit.is_pos lres); intro Heq; simpl; try now apply C.interp_true.
+    case_eq (t_form .[ Lit.blit lres]); try (intros; now apply C.interp_true).
+    intros a Heq2.
+    case_eq (length a == 2); [ intros Heq3 | intros Heq3; now apply C.interp_true].
+    case_eq (Lit.is_pos (a .[ 0]) && negb (Lit.is_pos (a .[ 1])));
+      [ intros Heq4 | intros Heq4; now apply C.interp_true].
+    case_eq (t_form .[ Lit.blit (a .[0])]); try (intros; now apply C.interp_true).
+    intros b Heq5.
+    case_eq (t_form .[ Lit.blit (a .[1])]); try (intros; now apply C.interp_true).
+    intros c Heq6.
+    case_eq (t_atom .[ b]); try (intros; now apply C.interp_true).
+    intros [ | | | | | | | |N|N|N|N|N|N|N|N|N| | | | ] b1 b2 Heq7; try (intros; now apply C.interp_true).
+    case_eq t; try (intros; now apply C.interp_true). intros t0 t1 Heq8.
+    case_eq (t_atom .[ c]); try (intros; now apply C.interp_true).
+    intros [ | | | | | | | |N|N|N|N|N|N|N|N|N| | | | ] c1 c2 Heq9; try (intros; now apply C.interp_true).
+    case_eq (Typ.eqb t1 t2); [ intros Heq10 | intros Heq10; now apply C.interp_true].
+    case_eq (t_atom .[ c1]); try (intros; now apply C.interp_true).
+    intros [ | | | | | | | |N|N|N|N|N|N|N|N|N| | | | ] d1 d2 Heq11; try (intros; now apply C.interp_true).
+    case_eq (t_atom .[ c2]); try (intros; now apply C.interp_true).
+    intros [ | | | | | | | |N|N|N|N|N|N|N|N|N| | | | ] e1 e2 Heq12; try (intros; now apply C.interp_true).
+    case_eq (t_atom .[ d2]);
+      try (intros; rewrite !andb_false_r; simpl; now apply C.interp_true).
+    intros [ | | | | | | | |N|N|N|N|N|N|N|N|N| | | | ] f1 f2 Heq14;
+      try (intros; rewrite !andb_false_r; simpl; now apply C.interp_true).
+    case_eq (Typ.eqb t0 t3 && Typ.eqb t0 t5 && Typ.eqb t1 t4 && Typ.eqb t1 t6);
+      [ intros Heq13'| intro; now apply C.interp_true].
+    simpl.
+    case_eq (Typ.eqb t0 t7 && Typ.eqb t1 t8);
+      [ intros Heq14'| intro; rewrite !andb_false_r; simpl; now apply C.interp_true].
+    simpl.
+    case_eq ((b1 == d1) && (b2 == e1) && (d2 == e2) && ((f1 == b1) && (f2 == b2))
+             || (b2 == d1) && (b1 == e1) && (d2 == e2) && ((f1 == b2) && (f2 == b1)));
+        [ intros Heq1314 | intro; now apply C.interp_true].
 
-      case_eq (Typ.eqb t0 t7 && Typ.eqb t1 t8 && (f1 == b1) && (f2 == b2)); 
-                [ intros Heq15 | intros Heq15; now apply C.interp_true].
+    unfold C.valid. simpl. rewrite orb_false_r.
 
-      unfold C.valid. simpl. rewrite orb_false_r.
+    rewrite orb_true_iff in Heq1314.
+    rewrite !andb_true_iff in Heq13'.
+    rewrite !andb_true_iff in Heq14'.
+    rewrite !andb_true_iff in Heq1314.
+    destruct Heq13' as (((Heq13, Heq13f), Heq13a), Heq13d).
+    destruct Heq14' as (Heq15, Heq15a).
 
-      rewrite !andb_true_iff in Heq13, Heq15.
-      destruct Heq13 as ((Heq13a, Heq13b), Heq13c).
-      rewrite andb_true_iff in Heq13a.
-      destruct Heq13a as ((Heq13a, Heq13d), Heq13e).
-      rewrite andb_true_iff in Heq13a.
-      destruct Heq13a as (Heq13, Heq13a).
-      rewrite andb_true_iff in Heq13.
-      destruct Heq13 as (Heq13, Heq13f).
+    apply Typ.eqb_spec in Heq13.
+    apply Typ.eqb_spec in Heq13f.
+    apply Typ.eqb_spec in Heq13a.
+    apply Typ.eqb_spec in Heq13d.
+    apply Typ.eqb_spec in Heq15.
+    apply Typ.eqb_spec in Heq15a.
+    subst t3 t5 t4 t6 t7 t8.
+    rewrite !Int63Properties.eqb_spec in Heq1314.
 
-      destruct Heq15 as (((Heq15, Heq15a), Heq15b), Heq15c).
+    unfold Lit.interp. rewrite Heq.
+    unfold Var.interp.
+    rewrite !wf_interp_form; trivial. rewrite Heq2. simpl.
+    rewrite afold_left_or.
+    unfold to_list.
+    rewrite Int63Properties.eqb_spec in Heq3.
+    rewrite Heq3.
 
-      apply Typ.eqb_spec in Heq13.
-      apply Typ.eqb_spec in Heq13f.
-      apply Typ.eqb_spec in Heq13a.
-      apply Typ.eqb_spec in Heq13d.
-      apply Typ.eqb_spec in Heq15.
-      apply Typ.eqb_spec in Heq15a.
+    (* for native-coq compatibility *)
+    assert (0 == 2 = false) as NCC.
+    { auto. } rewrite NCC.
+    (* simpl. *)
+    rewrite foldi_down_gt; auto.
 
-      apply Int63Properties.eqb_spec in Heq13e.
-      apply Int63Properties.eqb_spec in Heq13b.
-      apply Int63Properties.eqb_spec in Heq13c.
-      apply Int63Properties.eqb_spec in Heq15b.
-      apply Int63Properties.eqb_spec in Heq15c.
+    (* simpl. *)
+    assert (2 - 1 = 1). { auto. }
+                        rewrite H.
+    rewrite foldi_down_eq; auto. 
+    simpl. rewrite orb_false_r.
+    assert (1 - 1 = 0) as Has2. { auto. }
+                                rewrite Has2.
 
-      unfold Lit.interp. rewrite Heq.
-      unfold Var.interp.
-      rewrite !wf_interp_form; trivial. rewrite Heq2. simpl.
-      rewrite afold_left_or.
-      unfold to_list.
-      rewrite Int63Properties.eqb_spec in Heq3.
-      rewrite Heq3.
+    case_eq (Lit.interp rho (a .[ 0])). intro Hisa0.
+    rewrite orb_true_l. easy. intro Hisa. rewrite orb_false_l.
 
-      (* for native-coq compatibility *)
-      assert (0 == 2 = false) as NCC.
-      { auto. } rewrite NCC.
-      (* simpl. *)
-      rewrite foldi_down_gt; auto.
+    pose proof (rho_interp (Lit.blit (a .[ 0]))).
+    pose proof (rho_interp (Lit.blit (a .[ 1]))).
 
-      (* simpl. *)
-      assert (2 - 1 = 1). { auto. }
-      rewrite H.
-      rewrite foldi_down_eq; auto. 
-      simpl. rewrite orb_false_r.
-      assert (1 - 1 = 0) as Has2. { auto. }
-      rewrite Has2.
+    rewrite Heq5 in H0. rewrite Heq6 in H1.
+    simpl in H0, H1.
+    unfold Lit.interp.
+    rewrite andb_true_iff in Heq4.
+    destruct Heq4 as (Heq4, Heq4a).
+    apply negb_true_iff in Heq4a.
 
-      case_eq (Lit.interp rho (a .[ 0])). intro Hisa0.
-      rewrite orb_true_l. easy. intro Hisa. rewrite orb_false_l.
+    unfold Lit.interp in Hisa.
+    rewrite Heq4 in Hisa. unfold Var.interp in Hisa.
+    rewrite Hisa in H0. symmetry in H0.
+    rewrite Heq4a.
+    unfold Var.interp.
+    rewrite H1.
 
-      pose proof (rho_interp (Lit.blit (a .[ 0]))).
-      pose proof (rho_interp (Lit.blit (a .[ 1]))).
-
-      rewrite Heq5 in H0. rewrite Heq6 in H1.
-      simpl in H0, H1.
-      unfold Lit.interp.
-      rewrite andb_true_iff in Heq4.
-      destruct Heq4 as (Heq4, Heq4a).
-      apply negb_true_iff in Heq4a.
-
-      unfold Lit.interp in Hisa.
-      rewrite Heq4 in Hisa. unfold Var.interp in Hisa.
-      rewrite Hisa in H0. symmetry in H0.
-      rewrite Heq4a.
-      unfold Var.interp.
-      rewrite H1.
-
-      generalize wt_t_atom. unfold Atom.wt. unfold is_true.
-      rewrite PArray.forallbi_spec;intros.
+    generalize wt_t_atom. unfold Atom.wt. unfold is_true.
+    rewrite PArray.forallbi_spec;intros.
 
     (* b *)
-      pose proof (H2 b). assert (b < PArray.length t_atom).
-      apply PArray.get_not_default_lt. rewrite def_t_atom. rewrite Heq7. easy.
-      specialize (H3 H4). simpl in H3.
-      rewrite Heq7 in H3. simpl in H3.
-      rewrite !andb_true_iff in H3. destruct H3. destruct H3.
-      unfold get_type' in H3, H5, H6. unfold v_type in H3, H5, H6.
+    pose proof (H2 b). assert (b < PArray.length t_atom).
+    apply PArray.get_not_default_lt. rewrite def_t_atom. rewrite Heq7. easy.
+    specialize (H3 H4). simpl in H3.
+    rewrite Heq7 in H3. simpl in H3.
+    rewrite !andb_true_iff in H3. destruct H3. destruct H3.
+    unfold get_type' in H3, H5, H6. unfold v_type in H3, H5, H6.
 
-      case_eq (t_interp .[ b]).
-        intros v_typeb v_valb Htib. rewrite Htib in H3.
-        pose proof Htib as Htib''.
-        case_eq v_typeb; intros; rewrite H7 in H3; try now contradict H3.
+    case_eq (t_interp .[ b]).
+    intros v_typeb v_valb Htib. rewrite Htib in H3.
+    pose proof Htib as Htib''.
+    case_eq v_typeb; intros; rewrite H7 in H3; try now contradict H3.
 
-      case_eq (t_interp .[ b1]).
-        intros v_typeb1 v_valb1 Htib1. rewrite Htib1 in H6.
-        pose proof Htib1 as Htib1''.
-      case_eq (t_interp .[ b2]).
-          intros v_typeb2 v_valb2 Htib2. rewrite Htib2 in H5.
-        pose proof Htib2 as Htib2''.
-      rewrite Atom.t_interp_wf in Htib; trivial.
-      rewrite Atom.t_interp_wf in Htib1; trivial.
-      rewrite Atom.t_interp_wf in Htib2; trivial.
-      rewrite Heq7 in Htib. simpl in Htib.
-      rewrite !Atom.t_interp_wf in Htib; trivial.
-      rewrite Htib1, Htib2 in Htib.
-      unfold apply_binop in Htib.
-      apply Typ.eqb_spec in H5.
-      apply Typ.eqb_spec in H6.
+    case_eq (t_interp .[ b1]).
+    intros v_typeb1 v_valb1 Htib1. rewrite Htib1 in H6.
+    pose proof Htib1 as Htib1''.
+    case_eq (t_interp .[ b2]).
+    intros v_typeb2 v_valb2 Htib2. rewrite Htib2 in H5.
+    pose proof Htib2 as Htib2''.
+    rewrite Atom.t_interp_wf in Htib; trivial.
+    rewrite Atom.t_interp_wf in Htib1; trivial.
+    rewrite Atom.t_interp_wf in Htib2; trivial.
+    rewrite Heq7 in Htib. simpl in Htib.
+    rewrite !Atom.t_interp_wf in Htib; trivial.
+    rewrite Htib1, Htib2 in Htib.
+    unfold apply_binop in Htib.
+    apply Typ.eqb_spec in H5.
+    apply Typ.eqb_spec in H6.
 
-      generalize dependent v_valb1. generalize dependent v_valb2.
-      generalize dependent v_valb.
-      rewrite H5, H6, H7. rewrite !Typ.cast_refl. intros.
+    generalize dependent v_valb1. generalize dependent v_valb2.
+    generalize dependent v_valb.
+    rewrite H5, H6, H7. rewrite !Typ.cast_refl. intros.
 
-      specialize (Atom.Bval_inj2 t_i (Typ.Tbool) (Typ.i_eqb t_i t v_valb1 v_valb2) (v_valb)).
-      intros. specialize (H8 Htib).
+    specialize (Atom.Bval_inj2 t_i (Typ.Tbool) (Typ.i_eqb t_i t v_valb1 v_valb2) (v_valb)).
+    intros. specialize (H8 Htib).
 
-     (* c *)
-      pose proof (H2 c). assert (c < PArray.length t_atom).
-      apply PArray.get_not_default_lt. rewrite def_t_atom. rewrite Heq9. easy.
-      specialize (H9 H10). simpl in H9.
-      rewrite Heq9 in H9. simpl in H9.
-      rewrite !andb_true_iff in H9. destruct H9. destruct H9.
-      unfold get_type' in H9, H11, H12. unfold v_type in H9, H11, H12.
+    (* c *)
+    pose proof (H2 c). assert (c < PArray.length t_atom).
+    apply PArray.get_not_default_lt. rewrite def_t_atom. rewrite Heq9. easy.
+    specialize (H9 H10). simpl in H9.
+    rewrite Heq9 in H9. simpl in H9.
+    rewrite !andb_true_iff in H9. destruct H9. destruct H9.
+    unfold get_type' in H9, H11, H12. unfold v_type in H9, H11, H12.
 
-      case_eq (t_interp .[ c]).
-        intros v_typec v_valc Htic. rewrite Htic in H9.
-        pose proof Htic as Htic''.
-        case_eq v_typec; intros; rewrite H13 in H9; try now contradict H9.
+    case_eq (t_interp .[ c]).
+    intros v_typec v_valc Htic. rewrite Htic in H9.
+    pose proof Htic as Htic''.
+    case_eq v_typec; intros; rewrite H13 in H9; try now contradict H9.
 
-      case_eq (t_interp .[ c1]).
-        intros v_typec1 v_valc1 Htic1. rewrite Htic1 in H12.
-      case_eq (t_interp .[ c2]).
-          intros v_typec2 v_valc2 Htic2. rewrite Htic2 in H11.
-      rewrite Atom.t_interp_wf in Htic; trivial.
-      rewrite Atom.t_interp_wf in Htic1; trivial.
-      rewrite Atom.t_interp_wf in Htic2; trivial.
-      rewrite Heq9 in Htic. simpl in Htic.
-      rewrite !Atom.t_interp_wf in Htic; trivial.
-      rewrite Htic1, Htic2 in Htic. simpl in Htic.
+    case_eq (t_interp .[ c1]).
+    intros v_typec1 v_valc1 Htic1. rewrite Htic1 in H12.
+    case_eq (t_interp .[ c2]).
+    intros v_typec2 v_valc2 Htic2. rewrite Htic2 in H11.
+    rewrite Atom.t_interp_wf in Htic; trivial.
+    rewrite Atom.t_interp_wf in Htic1; trivial.
+    rewrite Atom.t_interp_wf in Htic2; trivial.
+    rewrite Heq9 in Htic. simpl in Htic.
+    rewrite !Atom.t_interp_wf in Htic; trivial.
+    rewrite Htic1, Htic2 in Htic. simpl in Htic.
 
-      apply Typ.eqb_spec in H11. apply Typ.eqb_spec in H12.
+    apply Typ.eqb_spec in H11. apply Typ.eqb_spec in H12.
 
-      generalize dependent v_valc1. generalize dependent v_valc2.
-      generalize dependent v_valc.
-      rewrite H11, H12, H13.
-      rewrite !Typ.cast_refl. intros. simpl in Htic.
-      unfold Bval in Htic.
+    generalize dependent v_valc1. generalize dependent v_valc2.
+    generalize dependent v_valc.
+    rewrite H11, H12, H13.
+    rewrite !Typ.cast_refl. intros. simpl in Htic.
+    unfold Bval in Htic.
 
-      specialize (Atom.Bval_inj2 t_i (Typ.Tbool) (Typ.i_eqb t_i t2 v_valc1 v_valc2) (v_valc)).
-      intros. specialize (H14 Htic).
+    specialize (Atom.Bval_inj2 t_i (Typ.Tbool) (Typ.i_eqb t_i t2 v_valc1 v_valc2) (v_valc)).
+    intros. specialize (H14 Htic).
 
-     (* c1 *)
-      pose proof (H2 c1). assert (c1 < PArray.length t_atom).
-      apply PArray.get_not_default_lt. rewrite def_t_atom. rewrite Heq11. easy.
-      specialize (H15 H16). simpl in H15.
-      rewrite Heq11 in H15. simpl in H15.
-      rewrite !andb_true_iff in H15. destruct H15. destruct H15.
-      unfold get_type' in H15, H17, H18. unfold v_type in H15, H17, H18.
+    (* c1 *)
+    pose proof (H2 c1). assert (c1 < PArray.length t_atom).
+    apply PArray.get_not_default_lt. rewrite def_t_atom. rewrite Heq11. easy.
+    specialize (H15 H16). simpl in H15.
+    rewrite Heq11 in H15. simpl in H15.
+    rewrite !andb_true_iff in H15. destruct H15. destruct H15.
+    unfold get_type' in H15, H17, H18. unfold v_type in H15, H17, H18.
 
-      case_eq (t_interp .[ c1]).
-        intros v_typec1' v_valc1' Htic1'. rewrite Htic1' in H15.
-        pose proof Htic1' as Htic1'''.
+    case_eq (t_interp .[ c1]).
+    intros v_typec1' v_valc1' Htic1'. rewrite Htic1' in H15.
+    pose proof Htic1' as Htic1'''.
 
-      case_eq (t_interp .[ d1]).
-        intros v_typed1 v_vald1 Htid1. rewrite Htid1 in H18.
-      case_eq (t_interp .[ d2]).
-          intros v_typed2 v_vald2 Htid2. rewrite Htid2 in H17.
-      rewrite Atom.t_interp_wf in Htic1'; trivial.
-      rewrite Atom.t_interp_wf in Htid1; trivial.
-      rewrite Atom.t_interp_wf in Htid2; trivial.
-      rewrite Heq11 in Htic1'. simpl in Htic1'.
-      rewrite !Atom.t_interp_wf in Htic1'; trivial.
-      rewrite Htid1, Htid2 in Htic1'. simpl in Htic1'.
+    case_eq (t_interp .[ d1]).
+    intros v_typed1 v_vald1 Htid1. rewrite Htid1 in H18.
+    case_eq (t_interp .[ d2]).
+    intros v_typed2 v_vald2 Htid2. rewrite Htid2 in H17.
+    rewrite Atom.t_interp_wf in Htic1'; trivial.
+    rewrite Atom.t_interp_wf in Htid1; trivial.
+    rewrite Atom.t_interp_wf in Htid2; trivial.
+    rewrite Heq11 in Htic1'. simpl in Htic1'.
+    rewrite !Atom.t_interp_wf in Htic1'; trivial.
+    rewrite Htid1, Htid2 in Htic1'. simpl in Htic1'.
 
-      apply Typ.eqb_spec in H15. apply Typ.eqb_spec in H17.
-      apply Typ.eqb_spec in H18.
+    apply Typ.eqb_spec in H15. apply Typ.eqb_spec in H17.
+    apply Typ.eqb_spec in H18.
 
-      generalize dependent v_vald1. generalize dependent v_vald2.
-      generalize dependent v_valc1'.
+    generalize dependent v_vald1. generalize dependent v_vald2.
+    generalize dependent v_valc1'.
 
-      rewrite H15, H17, H18.
-      unfold Bval. rewrite <- H15.
-      rewrite !Typ.cast_refl. intros.
+    rewrite H15, H17, H18.
+    unfold Bval. rewrite <- H15.
+    rewrite !Typ.cast_refl. intros.
 
-      specialize (Atom.Bval_inj2 t_i t4 (select v_vald1 v_vald2) (v_valc1')).
-      intros. specialize (H19 Htic1').
+    specialize (Atom.Bval_inj2 t_i t1 (select v_vald1 v_vald2) (v_valc1')).
+    intros. specialize (H19 Htic1').
 
-     (* c2 *)
-      pose proof (H2 c2). assert (c2 < PArray.length t_atom).
-      apply PArray.get_not_default_lt. rewrite def_t_atom. rewrite Heq12. easy.
-      specialize (H20 H21). simpl in H20.
-      rewrite Heq12 in H20. simpl in H20.
-      rewrite !andb_true_iff in H20. destruct H20. destruct H20.
-      unfold get_type' in H20, H22, H23. unfold v_type in H20, H22, H23.
+    (* c2 *)
+    pose proof (H2 c2). assert (c2 < PArray.length t_atom).
+    apply PArray.get_not_default_lt. rewrite def_t_atom. rewrite Heq12. easy.
+    specialize (H20 H21). simpl in H20.
+    rewrite Heq12 in H20. simpl in H20.
+    rewrite !andb_true_iff in H20. destruct H20. destruct H20.
+    unfold get_type' in H20, H22, H23. unfold v_type in H20, H22, H23.
 
-      case_eq (t_interp .[ c2]).
-        intros v_typec2' v_valc2' Htic2'. rewrite Htic2' in H20.
-        pose proof Htic2' as Htic2'''.
+    case_eq (t_interp .[ c2]).
+    intros v_typec2' v_valc2' Htic2'. rewrite Htic2' in H20.
+    pose proof Htic2' as Htic2'''.
 
-      case_eq (t_interp .[ e1]).
-        intros v_typee1 v_vale1 Htie1. rewrite Htie1 in H23.
-      case_eq (t_interp .[ e2]).
-          intros v_typee2 v_vale2 Htie2. rewrite Htie2 in H22.
-          pose proof Htie2 as Htie2''.
-      rewrite Atom.t_interp_wf in Htic2'; trivial.
-      rewrite Atom.t_interp_wf in Htie1; trivial.
-      rewrite Atom.t_interp_wf in Htie2; trivial.
-      rewrite Heq12 in Htic2'. simpl in Htic2'.
-      rewrite !Atom.t_interp_wf in Htic2'; trivial.
-      rewrite Htie1, Htie2 in Htic2'. simpl in Htic2'.
+    case_eq (t_interp .[ e1]).
+    intros v_typee1 v_vale1 Htie1. rewrite Htie1 in H23.
+    case_eq (t_interp .[ e2]).
+    intros v_typee2 v_vale2 Htie2. rewrite Htie2 in H22.
+    pose proof Htie2 as Htie2''.
+    rewrite Atom.t_interp_wf in Htic2'; trivial.
+    rewrite Atom.t_interp_wf in Htie1; trivial.
+    rewrite Atom.t_interp_wf in Htie2; trivial.
+    rewrite Heq12 in Htic2'. simpl in Htic2'.
+    rewrite !Atom.t_interp_wf in Htic2'; trivial.
+    rewrite Htie1, Htie2 in Htic2'. simpl in Htic2'.
 
-      apply Typ.eqb_spec in H20. apply Typ.eqb_spec in H22.
-      apply Typ.eqb_spec in H23.
+    apply Typ.eqb_spec in H20. apply Typ.eqb_spec in H22.
+    apply Typ.eqb_spec in H23.
 
-      generalize dependent v_valc1'. generalize dependent v_valc2'.
-      generalize dependent v_vale1. generalize dependent v_vale2.
+    generalize dependent v_valc1'. generalize dependent v_valc2'.
+    generalize dependent v_vale1. generalize dependent v_vale2.
 
-      rewrite H20, H22, H23.
-      unfold Bval. rewrite <- H20.
-      rewrite !Typ.cast_refl. intros.
+    rewrite H22. rewrite H20 in *. rewrite H23.
+    unfold Bval. rewrite <- H20.
+    rewrite !Typ.cast_refl. intros.
 
-      specialize (Atom.Bval_inj2 t_i t6 (select v_vale1 v_vale2) (v_valc2')).
-      intros. specialize (H24 Htic2').
+    specialize (Atom.Bval_inj2 t_i t1 (select v_vale1 v_vale2) (v_valc2')).
+    intros. specialize (H24 Htic2').
 
-     (* d2 *)
-      pose proof (H2 d2). assert (d2 < PArray.length t_atom).
-      apply PArray.get_not_default_lt. rewrite def_t_atom. rewrite Heq14. easy.
-      specialize (H25 H26). simpl in H25.
-      rewrite Heq14 in H25. simpl in H25.
-      rewrite !andb_true_iff in H25. destruct H25. destruct H25.
-      unfold get_type' in H25, H27, H28. unfold v_type in H25, H27, H28.
+    (* d2 *)
+    pose proof (H2 d2). assert (d2 < PArray.length t_atom).
+    apply PArray.get_not_default_lt. rewrite def_t_atom. rewrite Heq14. easy.
+    specialize (H25 H26). simpl in H25.
+    rewrite Heq14 in H25. simpl in H25.
+    rewrite !andb_true_iff in H25. destruct H25. destruct H25.
+    unfold get_type' in H25, H27, H28. unfold v_type in H25, H27, H28.
 
-      case_eq (t_interp .[ d2]).
-        intros v_typed2' v_vald2' Htid2'. rewrite Htid2' in H25.
-        pose proof Htid2' as Htid2'''.
+    case_eq (t_interp .[ d2]).
+    intros v_typed2' v_vald2' Htid2'. rewrite Htid2' in H25.
+    pose proof Htid2' as Htid2'''.
 
-      case_eq (t_interp .[ f1]).
-        intros v_typef1 v_valf1 Htif1. rewrite Htif1 in H28.
-      case_eq (t_interp .[ f2]).
-          intros v_typef2 v_valf2 Htif2. rewrite Htif2 in H27.
-      rewrite Atom.t_interp_wf in Htid2'; trivial.
-      rewrite Atom.t_interp_wf in Htif1; trivial.
-      rewrite Atom.t_interp_wf in Htif2; trivial.
-      rewrite Heq14 in Htid2'. simpl in Htid2'.
-      rewrite !Atom.t_interp_wf in Htid2'; trivial.
-      rewrite Htif1, Htif2 in Htid2'. simpl in Htid2'.
+    case_eq (t_interp .[ f1]).
+    intros v_typef1 v_valf1 Htif1. rewrite Htif1 in H28.
+    case_eq (t_interp .[ f2]).
+    intros v_typef2 v_valf2 Htif2. rewrite Htif2 in H27.
+    rewrite Atom.t_interp_wf in Htid2'; trivial.
+    rewrite Atom.t_interp_wf in Htif1; trivial.
+    rewrite Atom.t_interp_wf in Htif2; trivial.
+    rewrite Heq14 in Htid2'. simpl in Htid2'.
+    rewrite !Atom.t_interp_wf in Htid2'; trivial.
+    rewrite Htif1, Htif2 in Htid2'. simpl in Htid2'.
 
-      apply Typ.eqb_spec in H25. apply Typ.eqb_spec in H27.
-      apply Typ.eqb_spec in H28.
+    apply Typ.eqb_spec in H25. apply Typ.eqb_spec in H27.
+    apply Typ.eqb_spec in H28.
 
-      generalize dependent v_valf1. generalize dependent v_valf2.
-      generalize dependent v_vald2'.
+    generalize dependent v_valf1. generalize dependent v_valf2.
+    generalize dependent v_vald2'.
 
-      rewrite H25, H27, H28.
-      unfold Bval. rewrite <- H25.
-      rewrite !Typ.cast_refl. intros.
+    rewrite H25, H27, H28.
+    unfold Bval. rewrite <- H25.
+    rewrite !Typ.cast_refl. intros.
 
-      specialize (Atom.Bval_inj2 t_i t7 (diff v_valf1 v_valf2) (v_vald2')).
-      intros. specialize (H29 Htid2').
+    specialize (Atom.Bval_inj2 t_i t0 (diff v_valf1 v_valf2) (v_vald2')).
+    intros. specialize (H29 Htid2').
 
-     (* semantics *)
+    (* semantics *)
 
-      unfold Atom.interp_form_hatom, interp_hatom.
-      rewrite !Atom.t_interp_wf; trivial.
-      rewrite (*Heq7,*) Heq9. simpl.
-      rewrite !Atom.t_interp_wf; trivial.
-      rewrite (*Htib1, Htib2,*) Heq11, Heq12. simpl.
-      (*rewrite !Typ.cast_refl.*)
+    unfold Atom.interp_form_hatom, interp_hatom.
+    rewrite !Atom.t_interp_wf; trivial.
+    rewrite Heq9. simpl.
+    rewrite !Atom.t_interp_wf; trivial.
+    rewrite  Heq11, Heq12. simpl.
 
-      unfold apply_binop.
-      rewrite !Atom.t_interp_wf; trivial.
-      rewrite Htid1, Heq14, Htie1, Htie2.
-      rewrite !Typ.cast_refl.
-      simpl. (* (* native-coq compatibility *) unfold interp_atom. *)
-      rewrite !Atom.t_interp_wf; trivial.
-      rewrite Htif1, Htif2. simpl.
-      rewrite !Typ.cast_refl. simpl.
+    unfold apply_binop.
+    rewrite !Atom.t_interp_wf; trivial.
+    rewrite Htid1, Heq14, Htie1, Htie2.
+    rewrite !Typ.cast_refl.
+    simpl. (* (* native-coq compatibility *) unfold interp_atom. *)
+    rewrite !Atom.t_interp_wf; trivial.
+    rewrite Htif1, Htif2. simpl.
+    rewrite !Typ.cast_refl. simpl.
 
-      (* t7 = t3 *)
-      rewrite !Atom.t_interp_wf in Htid2'''; trivial.
-      rewrite Htid2 in Htid2'''.
-      inversion Htid2'''.
+    rewrite !Atom.t_interp_wf in Htid2'''; trivial.
+    rewrite Htid2 in Htid2'''.
+    inversion Htid2'''.
 
-      (* t2 = t6 *)
-      rewrite !Atom.t_interp_wf in Htic1'''; trivial.
-      rewrite Htic1 in Htic1'''.
-      inversion Htic1'''.
+    rewrite !Atom.t_interp_wf in Htic1'''; trivial.
+    rewrite Htic1 in Htic1'''.
+    inversion Htic1'''.
 
-      (* t4 = t6 *)
-      rewrite !Atom.t_interp_wf in Htic2'''; trivial.
-      rewrite Htic2 in Htic2'''.
-      inversion Htic2'''.
+    rewrite !Atom.t_interp_wf in Htic2'''; trivial.
+    rewrite Htic2 in Htic2'''.
+    inversion Htic2'''.
 
-      generalize dependent v_valc1. generalize dependent v_valc2.
-      generalize dependent v_valc1'. generalize dependent v_valc2'.
-      generalize dependent v_vald1. generalize dependent v_vald2.
+    generalize dependent v_valc1. generalize dependent v_valc2.
+    generalize dependent v_valc1'. generalize dependent v_valc2'.
+    generalize dependent v_vald1. generalize dependent v_vald2.
 
-      rewrite H31, H33.
-      rewrite !Typ.cast_refl. simpl.
-      rewrite !Typ.cast_refl.
-      rewrite H33 in H35. rewrite H35.
-      rewrite !Typ.cast_refl. intros. simpl.
+    subst.
+    rewrite !Typ.cast_refl. simpl.
+    rewrite !Typ.cast_refl. intros. simpl.
 
-      apply negb_true_iff.
-      apply Typ.i_eqb_spec_false.
+    apply negb_true_iff.
+    apply Typ.i_eqb_spec_false.
+    subst.
+    specialize (Atom.Bval_inj2 t_i v_typed2' (v_vald2) (diff v_valf1 v_valf2)).
+    intros. specialize (H5 Htid2''').
+    rewrite <- H5.
+    specialize (Atom.Bval_inj2 t_i v_typed2' (v_vale2) (v_vald2)).
+    intros.
 
-      generalize dependent v_vale1. generalize dependent v_vale2.
-      generalize dependent v_valf1. generalize dependent v_valf2.
+    unfold Atom.interp_form_hatom, interp_hatom in H0.
+    rewrite !Atom.t_interp_wf in H0; trivial.
+    rewrite Heq7 in H0. simpl in H0.
+    rewrite !Atom.t_interp_wf in H0; trivial.
+    rewrite Htib1, Htib2 in H0. simpl in H0.
+    rewrite !Typ.cast_refl in H0. simpl in H0.
+    apply Typ.i_eqb_spec_false in H0.
 
 
-      rewrite <- Heq15a, Heq13d.
-      rewrite <- Heq13f, Heq15. intros.
-      rewrite  H29.
+    destruct Heq1314 as [Heq1314 | Heq1314];
+      destruct Heq1314 as (((Heq13a, Heq13b), Heq13c), (Heq13d, Heq13e));
+      subst.
 
-      (* d2' = d2 *)
-      specialize (Atom.Bval_inj2 t_i t7 (v_vald2) (v_vald2')).
-      intros. specialize (H30 Htid2''').
-      rewrite <- H30.
-      (* d2 = e2 *)
-      rewrite Heq13c in Htid2.
-      rewrite Htie2 in Htid2.
-      specialize (Atom.Bval_inj2 t_i t7 (v_vale2) (v_vald2)).
-      intros. specialize (H37 Htid2).
-      rewrite H37.
-
-      (* b1 <> b2 *)
-      unfold Atom.interp_form_hatom, interp_hatom in H0.
-      rewrite !Atom.t_interp_wf in H0; trivial.
-      rewrite Heq7 in H0. simpl in H0.
-      rewrite !Atom.t_interp_wf in H0; trivial.
-      rewrite Htib1, Htib2 in H0. simpl in H0.
-      rewrite !Typ.cast_refl in H0. simpl in H0.
-      apply Typ.i_eqb_spec_false in H0.
-
-      (* f1 = b1 *)
-
-      generalize dependent v_vald1. generalize dependent v_vald2.
-      generalize dependent v_valc1'. generalize dependent v_valc2'.
-      generalize dependent v_vale1. generalize dependent v_vale2.
-
-      rewrite <- Heq13e, <- Heq13b; intros.
+    - rewrite Htie2 in Htid2.
       rewrite Htid1 in Htib1.
       rewrite Htie1 in Htib2.
-      inversion Htib1.
-      inversion Htib2.
+      rewrite Htid1 in Htif1.
+      rewrite Htie1 in Htif2.
 
-      generalize dependent v_valb.
-      generalize dependent v_valb1. generalize dependent v_valb2.
+      rewrite (Atom.Bval_inj2 t_i _ _ _ Htib1) in *.
+      rewrite (Atom.Bval_inj2 t_i _ _ _ Htib2) in *.
+      rewrite (Atom.Bval_inj2 t_i _ _ _ Htif1) in *.
+      rewrite (Atom.Bval_inj2 t_i _ _ _ Htif2) in *.
+      rewrite (Atom.Bval_inj2 t_i _ _ _ Htid2) in *.
 
-      rewrite <- H39. intros.
-      specialize (Atom.Bval_inj2 t_i (Typ.TFArray t7 t6) (v_vald1) (v_valb1)).
-      intros. specialize (H38 Htib1). rewrite H38.
-      specialize (Atom.Bval_inj2 t_i (Typ.TFArray t7 t6) (v_vale1) (v_valb2)).
-      intros. specialize (H43 Htib2). rewrite H43.
+      now apply select_at_diff.
 
-      rewrite H30, <- H29.
+    - rewrite Htie2 in Htid2.
+      rewrite Htid1 in Htib2.
+      rewrite Htie1 in Htib1.
+      rewrite Htid1 in Htif1.
+      rewrite Htie1 in Htif2.
 
-      (* b1 = f1 and b2 = f2 *)
-      rewrite Heq15b, Heq15c in *.
-      rewrite !Atom.t_interp_wf in Htib1''; trivial.
-      rewrite !Atom.t_interp_wf in Htib2''; trivial.
-      rewrite Htib1'' in Htif1.
-      rewrite Htib2'' in Htif2.
-      specialize (Atom.Bval_inj2 t_i (Typ.TFArray t7 t6) (v_valb1) (v_valf1)).
-      intros. specialize (H44 Htif1). rewrite H44.
-      specialize (Atom.Bval_inj2 t_i (Typ.TFArray t7 t6) (v_valb2) (v_valf2)).
-      intros. specialize (H45 Htif2). rewrite H45.
+      rewrite (Atom.Bval_inj2 t_i _ _ _ Htib1) in *.
+      rewrite (Atom.Bval_inj2 t_i _ _ _ Htib2) in *.
+      rewrite (Atom.Bval_inj2 t_i _ _ _ Htif1) in *.
+      rewrite (Atom.Bval_inj2 t_i _ _ _ Htif2) in *.
+      rewrite (Atom.Bval_inj2 t_i _ _ _ Htid2) in *.
 
       apply select_at_diff.
-      now rewrite H44, H45 in H0.
-      
-Qed.
-
+      red in H0. red. intro. apply H0. auto.
+  Qed.
+  
   End Correct.
 
 End certif.
